VCVio/OracleComp/OracleContext.lean
@@ -1,0 +1,36 @@
+/-
+Copyright (c) 2025 Devon Tuma. All rights reserved.
+Released under Apache 2.0 license as described in the file LICENSE.
+Authors: Devon Tuma
+-/
+import VCVio.OracleComp.SimSemantics.SimulateQ
+
+/-!
+# Bundled Oracle Specs and Implementations
+
+-/
+
+universe u v w z
+
+open OracleSpec OracleComp
+
+/-- An `OracleContext m` bundles an `OracleSpec` with an implementation of
+itself in terms of the monad `m`. This is useful for defining a shared interface
+in protocols where the execution method in protocol-dependent.
+
+A signature scheme for example could either include a random oracle or not,
+and set the appropriate behavior for the oracles in `OracleContext.impl`.-/
+structure OracleContext (m : Type v → Type w) :
+      Type (max u v w + 1) extends OracleSpec.{u,v}
+  where impl : QueryImpl toOracleSpec m
+
+namespace OracleContext
+
+/-- Simple `OracleContext` that implements the queries in the same
+overall `OracleComp spec` monad. -/
+def defaultContext (spec : OracleSpec.{u,v}) :
+    OracleContext (OracleComp spec) where
+  toOracleSpec := spec
+  impl := QueryImpl.id' spec
+
+end OracleContext
